theories/wasm_iris_use.v
@@ -1,0 +1,48 @@
+From iris.proofmode Require Import tactics.
+From iris.program_logic Require Export weakestpre.
+Require Export wasm_iris.
+Set Default Proof Using "Type". (* what is this? *)
+
+Record loc := { loc_car : Z }.
+Instance loc_eq_decision : EqDecision loc.
+Proof. solve_decision. Qed.
+
+Instance loc_inhabited : Inhabited loc := populate {|loc_car := 0 |}.
+
+Instance loc_countable : Countable loc.
+Proof. by apply (inj_countable' loc_car (λ i, {| loc_car := i |})); intros []. Qed.
+
+Program Instance loc_infinite : Infinite loc :=
+  inj_infinite (λ p, {| loc_car := p |}) (λ l, Some (loc_car l)) _.
+Next Obligation. done. Qed.
+
+
+Definition proph_id := positive.
+
+From iris.base_logic Require Export gen_heap.
+From iris.base_logic.lib Require Export proph_map.
+Class heapG Σ := HeapG {
+  heapG_invG : invG Σ;
+  heapG_gen_heapG :> gen_heapG loc val Σ;
+  heapG_proph_mapG :> proph_mapG proph_id (val * val) Σ
+}.
+
+Instance heapG_irisG `{!heapG Σ} : irisG wasm_lang Σ := {
+  iris_invG := heapG_invG;
+  state_interp σ κs _ := True%I
+(*    (gen_heap_ctx σ.(heap) ∗ proph_map_ctx κs σ.(used_proph_id))%I*);
+  fork_post _ := True%I;
+                                                       }.
+
+Definition xx i := (ConstInt32 (Wasm_int.int_of_nat (Wasm_int.mixin wasm.i32_r) i)).
+
+Definition my_add : wasm_iris.expr :=
+  [Basic (EConst (xx 3));
+     Basic (EConst (xx 2));
+     Basic (Binop_i T_i32 Add)].
+
+(* problem here :-( *)
+Lemma myadd_spec `{!heapG Σ} (s : stuckness) (E : coPset) (Φ : iProp Σ) (v : val) :
+  WP my_add @ s;E {{ fun v => exists v', v = xx 5 :: v' }}%I.
+Proof.
+Qed.
